theories/SLFAffine.v
@@ -1,0 +1,34 @@
+(**
+
+Separation Logic Foundations
+
+Chapter: "Affine".
+
+Author: Arthur Charguéraud.
+License: MIT.
+
+*)
+
+Set Implicit Arguments.
+From Sep Require Export SLFDirect.
+
+Implicit Types f : var.
+Implicit Types b : bool.
+Implicit Types v : val.
+Implicit Types h : heap.
+Implicit Types P : Prop.
+Implicit Types H : hprop.
+Implicit Types Q : val->hprop.
+
+
+(* ####################################################### *)
+(** * The chapter in a rush *)
+
+(** This chapter introduces the notion of weakest precondition
+    for Separation Logic triples. *)
+
+
+(* ******************************************************* *)
+(** ** Notion of weakest precondition *)
+
+
